# baseURI: https://models.bim4ren.eu/actors

@prefix : <https://models.bim4ren.eu/actors#> .
@prefix bot: <https://w3id.org/bot#> .
@prefix owl: <http://www.w3.org/2002/07/owl#> .
@prefix rdf: <http://www.w3.org/1999/02/22-rdf-syntax-ns#> .
@prefix rdfs: <http://www.w3.org/2000/01/rdf-schema#> .
@prefix xml: <http://www.w3.org/XML/1998/namespace> .
@prefix xsd: <http://www.w3.org/2001/XMLSchema#> .

<https://models.bim4ren.eu/actors>
  rdf:type owl:Ontology ;
  owl:versionIRI <https://models.bim4ren.eu/actors/0.1> ;
.
:ADULT
  rdf:type owl:NamedIndividual ;
  rdf:type :AgeCategory ;
  rdfs:comment "An adult is a person aged between 18 and 64 inclusive"@en ;
  rdfs:comment "Un adulte est une personne âgée antre 18 et 64 ans inclus"@fr ;
  rdfs:label "Adult"@en ;
  rdfs:label "Adulte"@fr ;
.
:Actor
  rdf:type owl:Class ;
  rdfs:comment "A building actor, which comes down to a building manager, a building owner or an occupant"@en ;
  rdfs:comment "Un acteur du bâtiment, qui peut être un maître d'oeuvre, un maître d'ouvrage ou un occupant"@fr ;
  rdfs:isDefinedBy "http://bsdd.buildingsmart.org/#concept/details/3xQru0qRmHuO00025QrE$V"@en ;
  rdfs:label "Acteur"@fr ;
  rdfs:label "Actor"@en ;
  rdfs:subClassOf [
      rdf:type owl:Restriction ;
      owl:maxQualifiedCardinality "1"^^xsd:nonNegativeInteger ;
      owl:onClass :AgeCategory ;
      owl:onProperty :ageCategory ;
    ] ;
.
:AgeCategory
  rdf:type owl:Class ;
  rdfs:comment "Correspond à une classification selon les tranches d'ages de personnes"@fr ;
  rdfs:comment "Corresponds to a classification according to people age groups"@en ;
  rdfs:label "Age category"@en ;
  rdfs:label "Catégorie d'âge"@fr ;
.
:BABY
  rdf:type owl:NamedIndividual ;
  rdf:type :AgeCategory ;
  rdfs:comment "A baby is a person who is less than a year old"@en ;
  rdfs:comment "Un bébé est une personne qui a moins d'un an"@fr ;
  rdfs:label "Baby"@en ;
  rdfs:label "Bébé"@fr ;
.
:BuildingManager
  rdf:type owl:Class ;
  rdfs:comment "Person or entity chosen by the building owner for the operational management of the work"@en ;
  rdfs:comment "Personne physique ou morale choisie par le maître d'ouvrage pour la conduite opérationnelle des travaux"@fr ;
  rdfs:label "Building manager"@en ;
  rdfs:label "Maître d'oeuvre"@fr ;
  rdfs:subClassOf :Actor ;
  owl:disjointWith :BuildingOwner ;
  owl:disjointWith :Occupant ;
.
:BuildingOwner
  rdf:type owl:Class ;
  rdfs:comment "Person or entity for whom the project is carried out"@en ;
  rdfs:comment "Personne physique ou morale pour laquelle le projet est réalisé"@fr ;
  rdfs:isDefinedBy "http://bsdd.buildingsmart.org/#concept/details/1B9uxpQzj5KBf25MREZyEH"@fr ;
  rdfs:label "Building owner"@en ;
  rdfs:label "Maître d'ouvrage"@fr ;
  rdfs:subClassOf :Actor ;
.
:CHILD
  rdf:type owl:NamedIndividual ;
  rdf:type :AgeCategory ;
  rdfs:comment "A child is a person aged between 1 year and 11 years inclusive"@en ;
  rdfs:comment "Un enfant est une personne âgée entre 1 an et 11 ans inclus"@fr ;
  rdfs:label "Child"@en ;
  rdfs:label "Enfant"@fr ;
.
:COMFORT
  rdf:type owl:NamedIndividual ;
  rdf:type :EnergyPolicy ;
  rdfs:comment "An occupant who is not eco friendly"@en ;
  rdfs:comment "Un occupant qui n'est pas éco-responsable"@fr ;
  rdfs:label "Comfort"@en ;
  rdfs:label "Comodidad"@es ;
  rdfs:label "Comodità"@it ;
  rdfs:label "Confort"@fr ;
.
:ECO
  rdf:type owl:NamedIndividual ;
  rdf:type :EnergyPolicy ;
  rdfs:comment "An occupant who is eco friendly"@en ;
  rdfs:comment "Un occupant éco-responsable"@fr ;
  rdfs:label "Eco friendly"@en ;
  rdfs:label "Eco-responsable"@fr ;
  rdfs:label "Ecológico"@es ;
  rdfs:label "Ecológico"@it ;
.
:ECO_PLUS
  rdf:type owl:NamedIndividual ;
  rdf:type :EnergyPolicy ;
  rdfs:comment "An occupant who is eco friendly++"@en ;
  rdfs:comment "Un occupant éco-responsable++"@fr ;
  rdfs:label "Eco friendly++"@en ;
  rdfs:label "Eco-responsable++"@fr ;
  rdfs:label "Ecológico++"@es ;
  rdfs:label "Ecológico++"@it ;
.
:ELDERLY
  rdf:type owl:NamedIndividual ;
  rdf:type :AgeCategory ;
  rdfs:comment "An elderly is a person aged 65 and over"@en ;
  rdfs:comment "Un personne âgée est une personne qui a 65 ans et plus"@fr ;
  rdfs:label "Elderly"@en ;
  rdfs:label "Personne âgée"@fr ;
.
:EMPLOYED
  rdf:type owl:NamedIndividual ;
  rdf:type :WorkType ;
  rdfs:comment "An occupant having a paid job"@en ;
  rdfs:comment "Un occupant ayant un emploi rémunéré"@fr ;
  rdfs:label "Employed"@en ;
  rdfs:label "Employé"@fr ;
.
:EnergyPolicy
  rdf:type owl:Class ;
  rdfs:comment "Defines to what extent the occupant pays attention to energy, and therefore has impacts on the heating or the use of certain devices during the simulation."@en ;
  rdfs:comment "Définit à quel point les occupants font attention ou non à l’énergie, et donc ont des impacts sur le chauffage ou l’utilisation de certains appareils durant la simulation. "@fr ;
  rdfs:label "Energy policy"@en ;
  rdfs:label "Politica energetica"@it ;
  rdfs:label "Politique énergétique"@fr ;
  rdfs:label "Política energética"@es ;
  owl:equivalentClass [
      rdf:type owl:Class ;
      owl:oneOf (
          :ECO
          :ECO_PLUS
          :COMFORT
        ) ;
    ] ;
.
:OccupancyProfile
  rdf:type owl:Class ;
  rdfs:comment "An occupancy profile describes some useful occupancy information (e.g., the occupancy time range) related to an occuppant associated to a given zone"@en ;
  rdfs:comment "Le profil d'occupation décrit certaines informations utiles (par exemple,les intervales d'occupation) liées à un occupant pour une zone donnée"@fr ;
  rdfs:label "Occupancy profile"@en ;
  rdfs:label "Profile d'occupation"@fr ;
  rdfs:subClassOf [
      rdf:type owl:Restriction ;
      owl:allValuesFrom :OccupancyTimeRange ;
      owl:onProperty :occupancyTime ;
    ] ;
  rdfs:subClassOf [
      rdf:type owl:Restriction ;
      owl:maxQualifiedCardinality "1"^^xsd:nonNegativeInteger ;
      owl:onClass bot:Zone ;
      owl:onProperty :associatedZone ;
    ] ;
.
:OccupancyTimeRange
  rdf:type owl:Class ;
  rdfs:comment "L'intervalle de temps d'occupation lié à un occupant et une zone donnée"@fr ;
  rdfs:comment "The occupancy time range related to an occupant and a given area"@en ;
  rdfs:label "Intervalle de temps d'occupation"@fr ;
  rdfs:label "Occupancy time range"@en ;
  rdfs:subClassOf [
      rdf:type owl:Restriction ;
      owl:allValuesFrom xsd:dateTime ;
      owl:onProperty :fromDateTime ;
    ] ;
  rdfs:subClassOf [
      rdf:type owl:Restriction ;
      owl:allValuesFrom xsd:dateTime ;
      owl:onProperty :toDateTime ;
    ] ;
.
:Occupant
  rdf:type owl:Class ;
  rdfs:comment "A type of actor that defines the form of occupancy of a property"@en ;
  rdfs:comment "Un type d'acteur qui définit la forme d'occupation d'une propriété"@fr ;
  rdfs:isDefinedBy "http://bsdd.buildingsmart.org/#concept/details/289KpOp8L4MBqIToXk2Uxq"@en ;
  rdfs:label "Occupant"@en ;
  rdfs:label "Occupant"@fr ;
  rdfs:subClassOf :Actor ;
  rdfs:subClassOf [
      rdf:type owl:Restriction ;
      owl:allValuesFrom :OccupancyProfile ;
      owl:onProperty :occupancyProfile ;
    ] ;
  rdfs:subClassOf [
      rdf:type owl:Restriction ;
      owl:allValuesFrom :WorkSituation ;
      owl:onProperty :workSituation ;
    ] ;
.
:SELF_EMPLOYED
  rdf:type owl:NamedIndividual ;
  rdf:type :WorkType ;
  rdfs:comment "An occupant who is working for oneself as a freelance or who is the owner of a business"@en ;
  rdfs:comment "Un occupant qui travaille pour soi-même en tant que freelance ou qui est le propriétaire d'une entreprise"@fr ;
  rdfs:label "Self employed"@en ;
  rdfs:label "Travailleur indépendant"@fr ;
.
:TEENAGER
  rdf:type owl:NamedIndividual ;
  rdf:type :AgeCategory ;
  rdfs:comment "A teenager is a person aged between 12 and 17 years inclusive"@en ;
  rdfs:comment "Un adolescent est une personne âgée entre 12 et 17 ans inclus"@fr ;
  rdfs:label "Adolescent"@fr ;
  rdfs:label "Teenager"@en ;
.
:UNEMPLOYED
  rdf:type owl:NamedIndividual ;
  rdf:type :WorkType ;
  rdfs:comment "An occupant without a paid job"@en ;
  rdfs:comment "Un occupant sans emploi"@fr ;
  rdfs:label "Unemployed"@en ;
  rdfs:label "sans emploi"@fr ;
.
:WorkSituation
  rdf:type owl:Class ;
  rdfs:comment "Describes the work situation of an occupant, mainly the type of work (if any), and its related income"@en ;
  rdfs:comment "Décrit la situation de travail d'un occupant, principalement le type de travail (le cas échéant) et son revenu"@fr ;
  rdfs:label "Situation de travail"@fr ;
  rdfs:label "Work situation"@en ;
  rdfs:subClassOf [
      rdf:type owl:Restriction ;
      owl:allValuesFrom xsd:decimal ;
      owl:onProperty :income ;
    ] ;
  rdfs:subClassOf [
      rdf:type owl:Restriction ;
      owl:allValuesFrom :WorkType ;
      owl:onProperty :workType ;
    ] ;
.
:WorkType
  rdf:type owl:Class ;
  rdfs:comment "Describes the occupant type of work"@en ;
  rdfs:comment "Décrit le type de travail d'un occupant"@fr ;
  rdfs:label "Type de travail"@fr ;
  rdfs:label "Work type"@en ;
  owl:equivalentClass [
      rdf:type owl:Class ;
      owl:oneOf (
          :EMPLOYED
          :SELF_EMPLOYED
          :UNEMPLOYED
        ) ;
    ] ;
.
:ageCategory
  rdf:type owl:ObjectProperty ;
  rdfs:comment "Relation describing the link between an actor and the corresponding age category"@fr ;
  rdfs:comment "Relation décrivant le lien entre un acteur et la catégorie d'âge correspondante"@fr ;
  rdfs:domain :Actor ;
  rdfs:label "age category"@en ;
  rdfs:label "catégorie d'âge"@fr ;
  rdfs:range :AgeCategory ;
.
:associatedActor
  rdf:type owl:ObjectProperty ;
  rdfs:comment "Relation describing the link between a zone and the associated actor, which could be the occupant or any actor having a specific role associated to the zone"@en ;
  rdfs:comment "Relation décrivant le lien entre une zone et un acteur associé, qui peut être l'occupant ou tout acteur ayant un rôle spécifique associé à cette zone"@fr ;
  rdfs:domain bot:Zone ;
  rdfs:label "acteur associé"@fr ;
  rdfs:label "associated actor"@en ;
  rdfs:range :Actor ;
.
:associatedZone
  rdf:type owl:ObjectProperty ;
  rdfs:comment "Relation pouvant décrire le lien entre un occupant et une zone associée à travers le profile d'occupation ou tout simplement le lien entre un acteur en général et une zone pour laquelle il a un role spécifique"@fr ;
  rdfs:comment "Relation that can describe the link between an occupant and an associated zone through the occupation profile or simply the link between an actor in general and a zone for which he has a specific role"@en ;
  rdfs:label "associated zone"@en ;
  rdfs:label "zone associée"@fr ;
  rdfs:range bot:Zone ;
.
:fromDateTime
  rdf:type owl:DatatypeProperty ;
  rdfs:comment "Property describing the start date and time related to an occupancy profile"@en ;
  rdfs:comment "Propriété décrivant la date et l'heure de début liées à un profil d'occupation"@fr ;
  rdfs:label "depuis date heure"@fr ;
  rdfs:label "from date time"@en ;
  rdfs:range xsd:dateTime ;
.
:hasEnergyPolicy
  rdf:type owl:ObjectProperty ;
  rdfs:comment "Property linking an occupant to the energy policy that he adopts"@en ;
  rdfs:comment "Propriété liant un occupant à la politique d'énergie qu'il adopte"@fr ;
  rdfs:domain :Occupant ;
  rdfs:label "energy policy"@en ;
  rdfs:label "politica energetica"@it ;
  rdfs:label "politique énergétique"@fr ;
  rdfs:label "política energética"@es ;
  rdfs:range :EnergyPolicy ;
.
:income
  rdf:type owl:DatatypeProperty ;
  rdfs:comment "Property describing the gross annual salary of an occupant"@en ;
  rdfs:comment "Propriété décrivant le salaire annuel brut d'un occupant"@fr ;
  rdfs:comment "salaire"@fr ;
  rdfs:label "income"@en ;
  rdfs:range xsd:decimal ;
.
:occupancyProfile
  rdf:type owl:ObjectProperty ;
  rdfs:comment "Relation describing the link between an occupant and its occupancy profile associated to a particular zone"@en ;
  rdfs:comment "Relation décrivant le lien entre un occupant et son profile d'occupation associé à une zone particulière"@fr ;
  rdfs:domain :Occupant ;
  rdfs:label "occupancy profile"@fr ;
  rdfs:label "profile d'occupation"@fr ;
  rdfs:range :OccupancyProfile ;
.
:occupancyTime
  rdf:type owl:ObjectProperty ;
  rdfs:comment "Relation describing the link between an occupancy profile (associated to an occupant and a given zone) and the corresponding occupancy time range"@en ;
  rdfs:comment "Relation décrivant le lien entre un profile d'occupation (associé à un occupant et une zone donnée) et l'intervalle d'occupation correspondant"@fr ;
  rdfs:domain :OccupancyProfile ;
  rdfs:label "occupancy time"@fr ;
  rdfs:label "temps d'occupation"@en ;
  rdfs:range :OccupancyTimeRange ;
.
:toDateTime
  rdf:type owl:DatatypeProperty ;
  rdfs:comment "Property describing the end date and time related to an occupancy profile"@en ;
  rdfs:comment "Propriété décrivant la date et l'heure de fin liées à un profil d'occupation"@fr ;
  rdfs:label "jusqu'au date heure"@fr ;
  rdfs:label "to date time"@en ;
  rdfs:range xsd:dateTime ;
.
:workSituation
  rdf:type owl:ObjectProperty ;
  rdfs:comment "Relation describing the link between an occupant and its work situation"@en ;
  rdfs:comment "Relation décrivant le lien entre un occupant et la situation de travail correspondate"@fr ;
  rdfs:domain :Occupant ;
  rdfs:label "situation de travail"@fr ;
  rdfs:label "work situation"@en ;
  rdfs:range :WorkSituation ;
.
:workType
  rdf:type owl:ObjectProperty ;
  rdfs:comment "Relation describing the link between a work situation associated to an occupant and the corresponding work type"@en ;
  rdfs:comment "Relation décrivant le lien entre la situation de travail associée à un occupant et le type de ce travail"@en ;
  rdfs:domain :WorkSituation ;
  rdfs:label "type de travail"@fr ;
  rdfs:label "work type"@en ;
  rdfs:range :WorkType ;
.
bot:Zone
  rdf:type owl:Class ;
.
